Lab 3

PfsProgs25/Labs/TreeMem.lean
@@ -28,13 +28,60 @@ The membership typeclass represents belonging to sets, lists and other collectio
 
 1. Define an instance of Membership in `BinTree α` corresponding to being a label. You may want to define an auxiliary function (or inductive type) first. (3 marks)
 -/
-instance {α: Type} : Membership α (BinTree α) := sorry
+def BinTree.containsLabel {α : Type} : (BinTree α) → α → Prop
+  | leaf a => fun label ↦ (label = a)
+  | node t₁ t₂ => fun label ↦ (containsLabel t₁ label) ∨ (containsLabel t₂ label)
+
+instance {α: Type} : Membership α (BinTree α) := Membership.mk BinTree.containsLabel
 
 /-!
 2. Prove that membership in a tree is equivalent to that in the corresponding list (3 marks).
 -/
-theorem mem_tree_iff_mem_list {α : Type} (tree : BinTree α ) :
-  ∀ x: α, x ∈ tree ↔ x ∈ tree.toList := by sorry
+theorem in_iff_containsLabel {α: Type} (tree : BinTree α) :
+  ∀ x: α, x ∈ tree ↔ tree.containsLabel x := by
+    intro x
+    simp [Membership.mem]
+
+theorem mem_tree_iff_mem_list {α : Type} (tree : BinTree α) :
+  ∀ elem : α, elem ∈ tree ↔ elem ∈ tree.toList := by
+  intro elem
+  induction tree with
+  | leaf value =>
+    rw [in_iff_containsLabel]
+    unfold BinTree.containsLabel
+    unfold BinTree.toList
+    simp
+  | node left right ih_left ih_right =>
+    constructor
+    · intro h
+      rw [in_iff_containsLabel] at h
+      unfold BinTree.containsLabel at h
+      unfold BinTree.toList
+      simp
+      cases h with
+      | inl hl =>
+        left
+        rw [← in_iff_containsLabel, ih_left] at hl
+        assumption
+      | inr hr =>
+        right
+        rw [← in_iff_containsLabel, ih_right] at hr
+        assumption
+    · intro h
+      rw [in_iff_containsLabel]
+      unfold BinTree.containsLabel
+      unfold BinTree.toList at h
+      simp at h
+      cases h with
+      | inl hl =>
+        left
+        rw [← in_iff_containsLabel, ih_left]
+        assumption
+      | inr hr =>
+        right
+        rw [← in_iff_containsLabel, ih_right]
+        assumption
+
 
 /-!
 ## Decidability
@@ -54,7 +101,14 @@ Decidable.isTrue : {p : Prop} → p → Decidable p
 /-!
 3. Using that membership in a List of natural numbers is decidable (or in some other way), construct an instance of the following. Note that a convenient way to use a decidable property is with an `if` statement of the form `if c:property then ... else ...`. (3 marks)
 -/
-instance {x: Nat}{t: BinTree Nat} : Decidable (x ∈ t) := sorry
+instance {x: Nat} {t: BinTree Nat} : Decidable (x ∈ t) := by
+  if h: x ∈ t.toList
+  then
+    rw [← mem_tree_iff_mem_list] at h
+    apply Decidable.isTrue h
+  else
+    rw [← mem_tree_iff_mem_list] at h
+    apply Decidable.isFalse h
 
 /-!
 As a test, uncomment the eval statements to get the appropriate results
@@ -62,8 +116,8 @@ As a test, uncomment the eval statements to get the appropriate results
 open BinTree in
 def eg₁ := node (node (leaf 3) (leaf 4)) (leaf 3)
 
--- #eval 3 ∈ eg₁
+#eval 3 ∈ eg₁
 
--- #eval 7 ∈ eg₁
+#eval 7 ∈ eg₁
 
 end lab
